theories/FOL/FOL.v
@@ -19,12 +19,12 @@ Inductive form : logic -> Type :=
 | All {b} : var -> form b -> form b.
 *)
 
-Inductive syms_func := t_f : bool -> syms_func | t_e.
+Inductive syms_func := s_f : bool -> syms_func | s_e.
 
 Instance sig_func : funcs_signature :=
   {| syms := syms_func; ar_syms := fun f => if f then 1 else 0 |}.
 
-Inductive syms_pred := Pr | Q.
+Inductive syms_pred := sPr | sQ.
 
 Instance sig_pred : preds_signature :=
   {| preds := syms_pred; ar_preds := fun P => if P then 2 else 0 |}.
